dafny/src/lendingProtocol.dfy
@@ -27,6 +27,7 @@ class LendingProtocol {
     var usersBalances: mapping<u160, u256>    // DAI
 
     const WAD: u256 := 1000000000000000000
+    const HALF_WAD: u256 := WAD / 2
 
     var DAI: ERC20
     var bDAI: ERC20
@@ -48,7 +49,7 @@ class LendingProtocol {
     }
     
 
-    method supply(msg: Transaction, amount: u256) returns (r: Result<()>)
+    method addCollateral(msg: Transaction, amount: u256) returns (r: Result<()>)
     modifies this`usersCollateral
     requires amount as nat <= MAX_U256 - usersCollateral.Get(msg.sender) as nat {
         usersCollateral := usersBalances.Set(msg.sender, usersCollateral.Get(msg.sender) + amount);
@@ -62,13 +63,28 @@ class LendingProtocol {
         return Ok(());
     }
 
+    method getExp(x: u256, y: u256) returns (result: u256)
+    requires x as nat * WAD as nat <= MAX_U256 as nat
+    requires y != 0
+    {
+        var mul: u256 := Mul(x, WAD);
+        result := Fixed.Div(mul, y);
+    }
+
+    method mulExp(x: u256, y: u256) returns (result: u256)
+    requires x as nat * y as nat <= MAX_U256 as nat
+    {
+        var mul: u256 := Mul(x, y);
+        assume {:axiom} (HALF_WAD as nat) + (mul as nat) <= MAX_U256 as nat;
+        var add: u256 := Add(HALF_WAD, mul);
+        result := Fixed.Div(add, WAD);
+    }
+
     method utilizationRatio() returns (utilizationRatio: u256)
-    requires this.fixedAnnuBorrowRate > this.baseRate
     requires this.totalBorrow as nat * WAD as nat <= MAX_U256 as nat
     requires this.totalDeposit != 0
     {
-        var mul: u256 := Mul(this.totalBorrow, WAD);
-        utilizationRatio := Fixed.Div(mul, this.totalDeposit);
+        utilizationRatio := getExp(this.totalBorrow, this.totalDeposit);
     }
 
     method interestMultiplier() returns (interestMul: u256)
@@ -78,12 +94,8 @@ class LendingProtocol {
     {
         var uRatio: u256 := utilizationRatio();
         var num: u256 := Sub(this.fixedAnnuBorrowRate, this.baseRate);
-        if uRatio == 0 {
-            interestMul := 0;
-        }
-        else {
-            interestMul := Fixed.Div(num, uRatio);
-        }
+        assume {:axiom} (uRatio as nat) > 0 as nat;
+        interestMul := getExp(num, uRatio);
     }
     
 
@@ -94,29 +106,65 @@ class LendingProtocol {
     {
         var uRatio: u256 := utilizationRatio();
         var interestMul: u256 := interestMultiplier();
-        var product:u256 :=0;
-        if uRatio as nat * interestMul as nat <= MAX_U256 as nat {
-            product := Mul(uRatio, interestMul);
-        }
-        rate := 0;
-        if product as nat + baseRate as nat <= MAX_U256 as nat {
-            rate := Add(product, baseRate);
-        }
+        assume {:axiom} (uRatio as nat) * (interestMul as nat) <= MAX_U256 as nat;
+        var product := mulExp(uRatio, interestMul);
+        assume {:axiom} (product as nat) + (baseRate as nat) <= MAX_U256 as nat;
+        rate := Add(product, baseRate);
     }
 
-    method calculateBorrowFee(amount: u256) returns (fee: u256, paid: u256)
-    requires this.fixedAnnuBorrowRate > this.baseRate
+    // method calculateBorrowFee(amount: u256) returns (fee: u256, paid: u256)
+    method calculateBorrowFee(amount: u256) returns (paid: u256)
     requires this.totalBorrow as nat * WAD as nat <= MAX_U256 as nat
     requires this.totalDeposit != 0
     {
         var borrowRate: u256 := borrowRate();
-        fee := 0;
-        if amount as nat * borrowRate as nat <= MAX_U256 as nat {
-            fee := Mul(amount, borrowRate);
-        }
-        paid := 0;
-        if amount as nat - fee as nat > 0 as nat {
-            paid := Sub(amount, fee);
-        }
+        assume {:axiom} (amount as nat) * (borrowRate as nat) <= MAX_U256 as nat;
+        var fee: u256 := Mul(amount, borrowRate);
+        assume {:axiom} (amount as nat) - (fee as nat) >= 0 as nat;
+        paid := Sub(amount, fee);
     }
 }
+
+
+// --- TESTS
+
+import opened Fixed
+import opened Number
+import opened Maps
+import opened Tx
+
+method {:test} testLendingProtocol() {
+    // Instantiate the LendingProtocol class
+    var protocol := new LendingProtocol();
+
+    // Set necessary values for totalDeposit and totalBorrow using setter methods
+    protocol.totalDeposit := 100; // Setting totalDeposit to 1 ether (for example)
+    protocol.totalBorrow := 100;   // Setting totalBorrow to 0.5 ether (for example)
+
+    // protocol.totalDeposit := 100;
+
+    assert protocol.totalDeposit == 100;
+    assert protocol.totalBorrow == 100;
+
+    // Define the amount for which the borrow fee needs to be calculated
+    var borrowAmount: u256 := 20; // Example borrow amount
+
+    // Declare variables to store the results
+    var fee: u256;
+    var paid: u256;
+
+    // Call the calculateBorrowFee method and store the results
+    paid := protocol.calculateBorrowFee(borrowAmount);
+
+    assert paid == 14;
+
+    // Print or assert the results to verify correctness
+    // print "Borrow Fee: ", fee, "\n";
+    // print "Amount Paid: ", paid, "\n";
+
+    // Optionally, you can include assertions to check expected values
+    // assert fee >= 0;
+    // assert paid == borrowAmount - fee;
+}
+
+
